%!TEX root = ../../../_main.tex
\section{Reducible case}
\label{sec:3rc-reducible-case}

\begin{lemm}
	\typedlabel{lemm:properties-of-wk-in-reducible-coxeter-groups}
	Let $(W, S_1 \dotcup S_2)$ be a reducible Coxeter system with $\ord(st) = 2$ for $s \in S_1, t \in S_2$. Let $\theta = \id$, $s_1,\ldots,s_m,s \in S_1$ and $t_1,\ldots,t_n,t \in S_2$. Then

	\begin{enumerate}
		\item $\ul s$ acts by twisted conjugation on $\ul s_1 \ldots \ul s_m \ul t_1 \ldots \ul t_n$ if and only if it acts by twisted conjugation on $\ul s_1 \ldots \ul s_m$,
		\item $\ul t$ acts by twisted conjugation on $\ul s_1 \ldots \ul s_m \ul t_1 \ldots \ul t_n$ if and only if it acts by twisted conjugation on $\ul t_1 \ldots \ul t_m$, and
		\item $\ul s_1 \ldots \ul s_m \ul t_1 \ldots \ul t_n \ul s = \ul s_1 \ldots \ul s_m \ul s \ul t_1 \ldots \ul t_n$.
	\end{enumerate}

	\begin{proof}
		We have $\ul s_1 \ldots \ul s_m \ul t_1 \ldots \ul t_n = t_{i_q} \cdots t_{i_1} s_{j_r} \cdots s_{j_1} s_1 \cdots s_m t_1 \cdots t_n$ for some well chosen indices $1 \leq i_1 < \ldots < i_q \leq m$ and $1 \leq j_1 < \ldots < j_r \leq n$.

		\begin{enumerate}
			\item We prove this by a straight forward chain of equivalences.
			\begin{align*}
						& s (\ul s_1 \ldots \ul s_m \ul t_1 \ldots \ul t_n) s  =  \ul s_1 \ldots \ul s_m \ul t_1 \ldots \ul t_n \\
				\iff	& s (t_{i_q} \cdots t_{i_1} s_{j_r} \cdots s_{j_1} s_1 \cdots s_m t_1 \cdots t_n) s  =  t_{i_q} \cdots t_{i_1} s_{j_r} \cdots s_{j_1} s_1 \cdots s_m t_1 \cdots t_n \\
				\iff	& (t_{i_q} \cdots t_{i_1} t_1 \cdots t_n) s s_{j_r} \cdots s_{j_1} s_1 \cdots s_m s  =  (t_{i_q} \cdots t_{i_1} t_1 \cdots t_n) s_{j_r} \cdots s_{j_1} s_1 \cdots s_m \\
				\iff	& s s_{j_r} \cdots s_{j_1} s_1 \cdots s_m s  =  s_{j_r} \cdots s_{j_1} s_1 \cdots s_m \\
				\iff	& s (\ul s_1 \ldots \ul s_m) s = \ul s_1 \ldots \ul s_m
			\end{align*}
			\item This part is almost the same as before.
			\begin{align*}
						& t (\ul s_1 \ldots \ul s_m \ul t_1 \ldots \ul t_n) t  =  \ul s_1 \ldots \ul s_m \ul t_1 \ldots \ul t_n \\
				\iff	& t (t_{i_q} \cdots t_{i_1} s_{j_r} \cdots s_{j_1} s_1 \cdots s_m t_1 \cdots t_n) t  =  t_{i_q} \cdots t_{i_1} s_{j_r} \cdots s_{j_1} s_1 \cdots s_m t_1 \cdots t_n \\
				\iff	& t t_{i_q} \cdots t_{i_1} t_1 \cdots t_n t (s_{j_r} \cdots s_{j_1} s_1 \cdots s_m)  =  t_{i_q} \cdots t_{i_1} t_1 \cdots t_n (s_{j_r} \cdots s_{j_1} s_1 \cdots s_m) \\
				\iff	& t t_{i_q} \cdots t_{i_1} t_1 \cdots t_n t  =  t_{i_q} \cdots t_{i_1} t_1 \cdots t_n \\
				\iff	& t (\ul t_1 \ldots \ul t_n) t = \ul t_1 \ldots \ul t_n
			\end{align*}
			Note that the last equivalence is not true in general. Suppose $v \in \ti{\theta}$ to be an arbitrary twisted expression. In general we cannot deduce the action of $\ul s$ on a subexpression of $v$ from the action of $\ul s$ on $v$ itself. But with the first part of this lemma we can first conclude that $\ul t_1$ acts by twisted conjugation on $e$ if and only if it acts by twisted conjugation on $\ul s_1 \ldots \ul s_m$. Again with the same argument $\ul t_2$ acts by twisted conjugation on $\ul t_1$ iff it acts by twisted conjugation on $\ul s_1 \ldots \ul s_m \ul t_1$ and so forth.
			\item To avoid having to repeat the proof for twisted conjugative and multiplicative action of $\ul s$ we set $s' = s$ if $\ul s$ acts by twisted conjugation and else $s' = e$.
			\begin{align*}
					& \ul s_1 \ldots \ul s_m \ul t_1 \ldots \ul t_n \ul s \\
				= \	& s' (t_{i_q} \cdots t_{i_1} s_{j_r} \cdots s_{j_1} s_1 \cdots s_m t_1 \cdots t_n) s \\
				= \	& t_{i_q} \cdots t_{i_1} (s' s_{j_r} \cdots s_{j_1} s_1 \cdots s_m s) t_1 \cdots t_n \\
				= \	& t_{i_q} \cdots t_{i_1} (s_1 \ldots \ul s_m \ul s) t_1 \cdots t_n \\
				= \	& s_1 \ldots \ul s_m \ul s \ul t_1 \ldots \ul t_n
			\end{align*}
			Again note that the last to equalities need the two previous parts of this lemma. \qedhere
		\end{enumerate}
	\end{proof}
\end{lemm}

\begin{coro}
	\typedlabel{coro:wk-of-reducible-coxeter-groups}
	Let $(W,S_1 \dotcup S_2)$ be Coxeter system with $\ord(st) = 2$ whenever $s \in S_1, t \in S_2$. In particular $W$ is reducible. Let $W := W_{S_1}$ and $W_2 := W_{S_2}$ be the parabolic subgroups of $W$ corresponding to $S_1$ and $S_2$. Then we have $Wk(W,\id) \cong Wk(W_1,\id) \times Wk(W_2,\id)$.

	\begin{proof}
		We denote the relation in $W$ (resp. in $W_1$, $W_2$) by $\preceq_W$ (resp. by $\preceq_{W_1}$, $\preceq_{W_2}$). By \ref{lemm:properties-of-wk-in-reducible-coxeter-groups} for every element $w \in \ti{\id}(W)$ we can find a twisted expression like $w = \ul s_1 \ldots \ul s_m \ul t_1 \ldots \ul t_n$ with $s \in S_1, t \in S_2$. Hence, the map
		$$ \varphi : \ti{\id}(W_1) \times \ti{\id}(W_2) \to \ti{\id}(W) : (\ul s_1 \ldots \ul s_m, \ul t_1 \ldots \ul t_n) \mapsto \ul s_1 \ldots \ul s_m \ul t_1 \ldots \ul t_n $$
		is surjective. The injectivity is due to \ref{prop:reducible-coxeter-systems-isomorph-to-parabolic-subgroups}. It remains to show that $\preceq_W$ satisfies \ref{defi:direct-product-of-posets}. Let $v_1,w_1 \in \ti{\id}(W_1)$, $v_2,w_2 \in \ti{\id}(W_2)$ and $v = v_1v_2 = \varphi(v_1,v_2), w = w_1w_2 = \varphi(w_1,w_2) \in \ti{\id}(W)$. Suppose $v_i \preceq_{W_i} w_i$ for $i=1,2$. Then we have
		\begin{align*}
			v_1	& = \ul s_1 \ldots \ul s_m, &
			w_1	& = \ul s_1 \ldots \ul s_m \ldots \ul s_{m'} = v_1 \ul s_{m+1} \ldots \ul s_{m'}, \\
			v_2	& = \ul t_1 \ldots \ul t_n \textrm{ and} &
			w_2	& = \ul t_1 \ldots \ul t_n \ldots \ul t_{n'} = v_2 \ul t_{n+1} \ldots \ul t_{n'}
		\end{align*}
		for some well chosen generators $s_i \in S_1, t_i \in S_2$ and $0 \leq m \leq m', 0 \leq n \leq n'$. Hence,
		\begin{align*}
			v	& = v_1 v_2 = \ul s_1 \ldots \ul s_m \ul t_1 \ldots \ul t_n \preceq_W \ul s_1 \ldots \ul s_m \ul t_1 \ldots \ul t_n \ul s_{m+1} \ldots \ul s_{m'} \ul t_{n+1} \ldots \ul t_{n'} \\
				& = \ul s_1 \ldots \ul s_m \ul s_{m+1} \ldots \ul s_{m'} \ul t_1 \ldots \ul t_n  \ul t_{n+1} \ldots \ul t_{n'} = w_1 w_2 = w.
		\end{align*}
		In return, suppose $v \preceq_W w$. Then we have
		\begin{align*}
			v	& = \ul s_1 \ldots \ul s_m \ul t_1 \ldots \ul t_n \textrm{ and} \\
			w	& = \ul s_1 \ldots \ul s_m \ul t_1 \ldots \ul t_n \ul s_{m+1} \ldots \ul s_{m'} \ul t_{n+1} \ldots \ul t_{n'}
		\end{align*}
		for some well chosen generators $s_i \in S_1, t_i \in S_2$ and $0 \leq m \leq m', 0 \leq n \leq n'$. Again with similar arguments we have 
		\begin{align*}
			v_1	& = \ul s_1 \ldots \ul s_m \preceq_{W_1} \ul s_1 \ldots \ul s_m \ul s_{m+1} \ldots \ul s_{m'} = w_1 \textrm{ and} \\
			w_1	& = \ul t_1 \ldots \ul t_n \preceq_{W_2} \ul t_1 \ldots \ul t_n \ul t_{n+1} \ldots \ul t_{n'} = w_2. \qedhere
		\end{align*}
	\end{proof}
\end{coro}

\begin{rema}
	Note that \ref{lemm:properties-of-wk-in-reducible-coxeter-groups} and \ref{coro:wk-of-reducible-coxeter-groups} still hold if we drop the premise $\theta = \id$ and instead insist on $\theta(S_i) = S_i$ for $i=1,2$. They also remain true if we have a partition of the generator set in more than two subsets. Hence, for $(W,S_1 \dotcup \ldots \dotcup S_n)$ with $\ord(st) = 2$ whenever $s \in S_i, t \in S_j, i \neq j$ we have
	$$ Wk(W,\id) = Wk(W_{S_1},\id) \times \ldots \times Wk(W_{S_n},\id). $$
\end{rema}

\begin{theo}
	Let $(W,S)$ be a reducible Coxeter system with $S = S' \cup S''$ and $\ord(st) = 2$ whenever $s \in S', t \in S''$ and let $\theta = \id$. Then $Wk(W,\id)$ is 3-residually connected if and only if $Wk(W_{S'},\id)$ and $Wk(W_{S''},\id)$ are 3-residually connected.

	\begin{proof}
		If $Wk(W,\id)$ is 3-residually connected, then $Wk(W_{S'},\id)$ and $Wk(W_{S''},\id)$ are so in particular. In return, suppose $Wk(W_{S'},\id)$ and $Wk(W_{S''},\id)$ to be 3-residually connected. For a set $M \subseteq S$ we define $M' := M \cap S'$ and $M'' := M \cap S''$, hence $M = M' \dotcup M''$. This is compatible with our definition of $S_{ij}$ and $T$:
		\begin{align*}
			S_{ij}	& = S_i \cap S_j = (S'_i \dotcup S''_i) \cap (S'_j \dotcup S''_j) = (S'_i \cap S'_j) \dotcup (S''_i \cap S''_j) = S'_{ij} \dotcup S''_{ij} \\
			T		& = S_1 \cap S_2 \cap S_3 = (S'_{12} \dotcup S''_{12}) \cap (S'_3 \dotcup S''_3) = (S'_{12} \cap S'_3) \dotcup (S''_{12} \cap S''_3) = T' \dotcup T''
		\end{align*}
		Let $w_K = \ul s'_1 \ldots \ul s'_{m'} \ul s''_1 \ldots \ul s''_{m''}$ with $s'_i \in K',s''_i \in K''$. Then
		$w_{K'} = \ul s'_1 \ldots \ul s'_{m'}$ (resp. $w_{K''} = \ul s''_1 \ldots \ul s''_{m''}$) is the corresponding longest element in $\langle K' \rangle \leq W_{S'} \leq W$ (resp. $\langle K'' \rangle \leq W_{S''} \leq W$).
		We have three twisted expressions
		\begin{align*}
			w	& = w_K \ul a'_1 \ldots \ul a'_{n'} \ul a''_1 \ldots \ul a''_{n''} \\
				& = w_K \ul b'_1 \ldots \ul b'_{n'} \ul b''_1 \ldots \ul b''_{n''} \\
				& = w_K \ul c'_1 \ldots \ul c'_{n'} \ul c''_1 \ldots \ul c''_{n''}
		\end{align*}
		with $a'_i,a''_i \in S_1$, $b'_i,b''_i \in S_2$ and $c'_i,c''_i \in S_3$. Thanks to \ref{lemm:properties-of-wk-in-reducible-coxeter-groups} we can assume without loss of generality that $a',b',c' \in S'$ and $a'',b'',c'' \in S''$. Hence, we have also
		\begin{align*}
			w'	& = w_{K'} \ul a'_1 \ldots \ul a'_{n'} = s'_1 \ldots \ul s'_m \ul a'_1 \ldots \ul a'_{n'} \\
				& = w_{K'} \ul b'_1 \ldots \ul b'_{n'} = s'_1 \ldots \ul s'_m \ul b'_1 \ldots \ul b'_{n'} \\
				& = w_{K'} \ul c'_1 \ldots \ul c'_{n'} = s'_1 \ldots \ul s'_m \ul c'_1 \ldots \ul c'_{n'}
		\end{align*}
		and so $w' \in w_{K'}C_{T'}$, since \axiomref{3RC} holds in $Wk(W_{S'},\id)$. Analogue we get $w'' \in w_{K''}C_{T''}$. Hence,
		$$ w' = \ul s'_1 \ldots \ul s'_{m'} \ul d'_1 \ldots \ul d'_{l'} \textrm{ and } w'' = \ul s''_1 \ldots \ul s''_{m''} \ul d''_1 \ldots \ul d''_{l''} $$
		for $d'_i \in T'$ and $d''_i \in T''$. This yields a twisted expression
		\begin{align*}
			w	& = w' w'' = \ul s'_1 \ldots \ul s'_{m'} \ul d'_1 \ldots \ul d'_{l'} \ul s''_1 \ldots \ul s''_{m''} \ul d''_1 \ldots \ul d''_{l''} \\
				& = \ul s'_1 \ldots \ul s'_{m'} \ul s''_1 \ldots \ul s''_{m''} \ul d'_1 \ldots \ul d'_{l'} \ul d''_1 \ldots \ul d''_{l''} \\
				& = w_K \ul d'_1 \ldots \ul d'_{l'} \ul d''_1 \ldots \ul d''_{l''}
		\end{align*}
		with $d'_i,d''_i \in T' \dotcup T'' = T$. Thus $w \in w_KC_T$.
	\end{proof}
\end{theo}